make swap monomorphic

examples/steel/arraystructs/PointStruct.fst
@@ -66,22 +66,12 @@ let x_conn
 noextract
 let point = struct "point" point_fields
 
-assume
-val opt_drop
-  (#inames: _)
-  (#a: Type u#0) (#b: Type u#0)
-  (r: ref a (opt_pcm #b))
-: SteelGhostT unit inames
-  (pts_to_view r (opt_view b))
-  (fun _ -> emp)
-
-
 open Steel.C.Reference
 
-val swap (p: ref 'a point point_pcm)
-: Steel unit
+val swap (p: ref int point point_pcm)
+: Steel int
     (p `pts_to_view` point_view emptyset)
-    (fun _ -> emp) // (p `pts_to_view` point_view emptyset))
+    (fun _ -> p `pts_to_view` point_view emptyset)
     (requires fun _ -> True)
     (ensures fun h q h' -> True)
       // h' (p `pts_to_view` point_view emptyset) `struct_get` "x"
@@ -89,20 +79,17 @@ val swap (p: ref 'a point point_pcm)
       // h' (p `pts_to_view` point_view emptyset) `struct_get` "y"
       // == h (p `pts_to_view` point_view emptyset) `struct_get` "x")
 
-let swap #a p =
+let swap p =
   let q: ref _ int _ = addr_of_struct_field "x" p in
-  opt_drop q;
   let r: ref _ int _ = addr_of_struct_field "y" p in
-  opt_drop r;
-  drop (p `pts_to_view` _);
-  // let x = opt_read_sel q in
-  // let y = opt_read_sel r in
-  // q `opt_write_sel` y;
-  // r `opt_write_sel` x;
-  // unaddr_of_struct_field "y" p r;
-  // unaddr_of_struct_field "x" p q;
-  // change_equal_slprop (p `pts_to_view` _) (p `pts_to_view` _);
-  return ()
+  let x = opt_read_sel q in
+  let y = opt_read_sel r in
+  q `opt_write_sel` y;
+  r `opt_write_sel` x;
+  unaddr_of_struct_field "y" p r;
+  unaddr_of_struct_field "x" p q;
+  change_equal_slprop (p `pts_to_view` _) (p `pts_to_view` _);
+  return 42
 
 (*
 ref 'a (struct tag fields)
